A simple symbolic evaluation.

MirrorCharge!/src/Imp/SymEval.v
@@ -1,59 +1,149 @@
+Require Import BinPos.
 Require Import MirrorCore.Lemma.
-Require Import MirrorCore.Lambda.TypesI2.
+Require Import MirrorCore.TypesI.
 Require Import MirrorCore.Lambda.Expr.
-Require Import McExamples.STac.STac.
-Require Import MirrorCharge.ILogicFunc.
+Require Import MirrorCore.STac.STac.
+Require Import MirrorCore.provers.DefaultProver.
+Require MirrorCore.syms.SymEnv.
+Require Import MirrorCore.Subst.FMapSubst3.
+Require Import MirrorCore.Lambda.ExprLift.
+Require Import MirrorCore.Lambda.ExprSubst.
+Require Import MirrorCore.Lambda.ExprUnify_simul.
 Require Import MirrorCharge.Imp.Imp.
 
 Set Implicit Arguments.
 Set Strict Implicit.
 
+Definition func := SymEnv.func.
+
+Inductive typ :=
+| tyArr : typ -> typ -> typ
+| tyLocals : typ
+| tyCmd : typ
+| tyHProp : typ
+| tyProp : typ.
+
+Fixpoint typD (ls : list Type) (t : typ) : Type :=
+  match t with
+    | tyArr a b => typD ls a -> typD ls b
+    | tyLocals => locals
+    | tyCmd => icmd
+    | tyHProp => HProp
+    | tyProp => Prop
+  end.
+
+Inductive tyAcc_typ : typ -> typ -> Prop :=
+| tyAcc_tyArrL : forall a b, tyAcc_typ a (tyArr a b)
+| tyAcc_tyArrR : forall a b, tyAcc_typ a (tyArr b a).
+
+Fixpoint type_cast_typ (a b : typ) : option (a = b) :=
+  match a as a , b as b return option (a = b) with
+    | tyLocals , tyLocals => Some eq_refl
+    | tyCmd , tyCmd => Some eq_refl
+    | tyHProp , tyHProp => Some eq_refl
+    | tyProp , tyProp => Some eq_refl
+    | tyArr x y , tyArr a b =>
+      match type_cast_typ x a , type_cast_typ y b with
+        | Some pf , Some pf' =>
+          Some (match pf in _ = t
+                    , pf' in _ = t'
+                      return tyArr x y = tyArr t t'
+                with
+                  | eq_refl , eq_refl => eq_refl
+                end)
+        | _ , _ => None
+      end
+    | _ , _ => None
+  end.
+
+Instance RType_typ : RType typ :=
+{ typD := typD
+; tyAcc := tyAcc_typ
+; type_cast := fun _ => type_cast_typ
+}.
+
+Instance Typ2_Fun : Typ2 _ Fun :=
+{ typ2 := tyArr
+; typ2_cast := fun _ _ _ => eq_refl
+; typ2_match := fun T ts t tr =>
+                  match t as t return T (typD ts t) -> T (typD ts t) with
+                    | tyArr a b => fun _ => tr a b
+                    | _ => fun fa => fa
+                  end
+}.
+
+
 Section tactic.
-  Variable RType_typ : TypesI2.RType.
-  Variable Typ2_arr : Typ2 _ Fun.
-  Variable subst : Type.
-  
-  Let tyArr : typ -> typ -> typ := @typ2 _ _ _.
+  Let subst : Type :=
+    @FMapSubst3.SUBST.raw (expr typ func).
+  Instance SS : SubstI3.Subst subst (expr typ func) :=
+    FMapSubst3.SUBST.Subst_subst _.
+  Instance SU : SubstI3.SubstUpdate subst (expr typ func) :=
+    FMapSubst3.SUBST.SubstUpdate_subst (@mentionsU typ func)
+                                       (@instantiate typ func).
 
-  Axiom tyLocals : typ.
-  Axiom tyCmd : typ.
-  Axiom tyHProp : typ.
-  Axiom tyProp : typ.
+  Let tyLProp := tyArr tyLocals tyHProp.
 
-  Axiom fTriple : expr typ ilfunc.
-  Axiom fSeq : expr typ ilfunc.
+  Let fs : @SymEnv.functions typ _ :=
+    SymEnv.from_list
+      (@SymEnv.F typ _ (tyArr tyLProp (tyArr tyCmd (tyArr tyLProp tyProp)))
+                 (fun _ => triple) ::
+       @SymEnv.F typ _ (tyArr tyCmd (tyArr tyCmd tyCmd))
+                 (fun _ => Seq) ::
+       nil).
 
-  Definition mkTriple (P c Q : expr typ ilfunc) : expr typ ilfunc :=
+  Definition RS : SymI.RSym func := SymEnv.RSym_func fs.
+  Definition EP : EProver2.EProver (typ := typ) (expr typ func) :=
+    EProver2.from_Prover (DefaultProver (expr typ func)).
+
+  Let tyArr : typ -> typ -> typ := @typ2 _ _ _ _.
+
+  Definition fTriple : expr typ func := Inj 1%positive.
+  Definition fSeq : expr typ func := Inj 2%positive.
+
+  Definition mkTriple (P c Q : expr typ func) : expr typ func :=
     App (App (App fTriple P) c) Q.
-  Definition mkSeq (a b : expr typ ilfunc) : expr typ ilfunc :=
+  Definition mkSeq (a b : expr typ func) : expr typ func :=
     App (App fSeq a) b.
 
-  Definition seq_lemma : lemma typ (expr typ ilfunc) (expr typ ilfunc) :=
+  (** NOTE: Manual lemma reification for the time being **)
+  Definition seq_lemma : lemma typ (expr typ func) (expr typ func) :=
   {| vars := tyArr tyLocals tyHProp :: tyArr tyLocals tyHProp ::
              tyArr tyLocals tyHProp :: tyCmd :: tyCmd :: nil
    ; premises := mkTriple (Var 4) (Var 1) (Var 3) ::
-                mkTriple (Var 3) (Var 0) (Var 2) :: nil
+                 mkTriple (Var 3) (Var 0) (Var 2) :: nil
    ; concl := mkTriple (Var 4) (mkSeq (Var 1) (Var 0)) (Var 2)
    |}.
 
-  Definition seq_assoc_lemma : lemma typ (expr typ ilfunc) (expr typ ilfunc) :=
+  Definition seq_assoc_lemma : lemma typ (expr typ func) (expr typ func) :=
   {| vars := tyArr tyLocals tyHProp :: tyArr tyLocals tyHProp ::
              tyCmd :: tyCmd :: tyCmd :: nil
-   ; premises := mkTriple (Var 4) (mkSeq (Var 2) (mkSeq (Var 1) (Var 0))) (Var 3) :: nil
-   ; concl := mkTriple (Var 4) (mkSeq (mkSeq (Var 2) (Var 1)) (Var 0)) (Var 3)
+   ; premises :=
+       mkTriple (Var 0) (mkSeq (Var 2) (mkSeq (Var 3) (Var 4))) (Var 1) :: nil
+   ; concl :=
+       mkTriple (Var 0) (mkSeq (mkSeq (Var 2) (Var 3)) (Var 4)) (Var 1)
    |}.
 
-  Require Import MirrorCore.Lambda.ExprLift.
-  Require Import MirrorCore.Lambda.ExprUnify_simul.
-
   Let eapply_other :=
-    @eapply_other typ (expr typ ilfunc) subst tyProp vars_to_uvars.
-  Check eapply_other.
-  Check exprUnify.
-  Check (@exprUnify subst ilfunc _ _).
+    @eapply_other typ (expr typ func) subst tyProp vars_to_uvars
+                  (fun tus tvs n e1 e2 t s =>
+                     @exprUnify subst typ func _ _ RS SS SU 1 nil
+                                tus tvs n s e1 e2 t) SS SU.
 
-
-  Definition seq_case : branch typ (expr typ ilfunc) subst :=
-    FIRST (   eapply_other seq_assoc_lemma _
-           :: eapply_other seq_lemma _
+  Definition seq_case : branch typ (expr typ func) subst :=
+    FIRST (   eapply_other seq_assoc_lemma EP
+           :: eapply_other seq_lemma EP
            :: nil).
+
+  Let goal : expr typ func :=
+    mkTriple (Var 0)
+             (mkSeq (mkSeq (Var 1) (Var 2)) (Var 3))
+             (Var 4).
+
+  Definition test :=
+    @seq_case goal (SubstI3.empty (expr :=expr typ func))
+              nil (tyLProp :: tyCmd :: tyCmd :: tyCmd :: tyLProp :: nil).
+
+  Time Eval vm_compute in test.
+
+End tactic.
